src/util/StateMonad.v
@@ -17,81 +17,22 @@ Definition ctr_bnd {a b: Type} (f: a -> ctr b) (x: ctr a) : ctr b :=
 Definition new_ctr : ctr unit := fun _ => (CoqBigInt.zero, tt).
 Definition incr : ctr unit := fun i => (CoqBigInt.succ i, tt).
 
+(*TODO: remove*)
 From stdpp Require Import base.
 Global Instance ctr_ret': MRet ctr := @ctr_ret.
 Global Instance ctr_bnd': MBind ctr := @ctr_bnd.
 
+(*A vile hack - for extraction, we need a type that does not
+  get erased when creating a counter*)
+Definition ctr_unit := ctr unit.
 
-(*Definition st_bnd {s a b: Type} (f: a -> state s b) (x: state s a) : state s b :=
-  fun s => 
-    let t := runState x s in
-    runState (f (snd t)) (fst t).
-
-
-Definition ctr_bind
-
-
-(*We want a mutable counter to register identifiers*)
-
-(*We offer a very restricted interface so that we can
-  extract to OCaml mutable references soundly*)
-
-Definition state (s: Type) (a: Type) : Type := s -> s * a.
-Definition runState {s a} (x: state s a) : s -> s * a := x.
-
-Definition st_ret {s a} (x: a) : state s a :=
-  fun s => (s, x).
-
-Definition get {s: Type} : state s s :=
-  fun s => (s, s).
-Definition put {s: Type} (x: s) : state s unit :=
-  fun _ => (x, tt).
-Definition evalState {s a: Type} (x: state s a) (y: s) : a :=
-  snd (x y).
-Definition execState {s a: Type} (x: state s a) (y: s) : s :=
-  fst (x y).
-
-Definition st_bnd {s a b: Type} (f: a -> state s b) (x: state s a) : state s b :=
-  fun s => 
-    let t := runState x s in
-    runState (f (snd t)) (fst t).
-
-From stdpp Require Import base.
-Global Instance state_ret {s: Type}: MRet (state s) := @st_ret s.
-Global Instance errorM_bind {s: Type}: MBind (state s) := @st_bnd s.
-
-
-(*For now, only 1 global counter/int that is stored
-  TODO: see if we need others*)
-Require CoqBigInt.
-Definition ctr (a: Type) := state CoqBigInt.t a.
-Definition new_ctr {a: Type} (i: CoqBigInt.t) (x: a) : ctr a :=
-  fun _ => (i, x).
-Definition incr : ctr unit :=
-  fun i => (CoqBigInt.succ i, tt).
-  (*ONLY through this interface!*)
-  
-
-
-
-
-
-(*Axiom ST : Type -> Type -> Type.
-Axiom runST : forall (a: Type), (forall s, ST s a) -> a.
-Axiom bnd : forall (s a b: Type), ST s a -> (a -> ST s b) -> ST s b.
-Axiom ret: forall (s a: Type), a -> ST s a.
-
-Axiom STRef : Type -> Type -> Type.
-Axiom newSTRef : forall (s a: Type), a -> ST s (STRef s a).
-Axiom readSTRef : forall (s a: Type), STRef s a -> ST s a.
-Axiom writeSTRef: forall (s a: Type), STRef s a -> a -> ST s unit.
-Axiom modifySTRef: forall (s a: Type), STRef s a -> (a -> a) -> ST s unit.
-
-(*A counter*)
-Require CoqBigInt.
-Definition new_ctr (s: Type) : ST s (STRef s CoqBigInt.t) :=
-  newSTRef s _ (CoqBigInt.zero).
-Definition incr (s: Type) (ctr: STRef s CoqBigInt.t) : 
-  ST s (STRef s CoqBigInt.t) :=
-  modifySTRef _ _ ctr CoqBigInt.succ.
-  bnd _ _ _ ctr (fun x => ret _ _ (CoqBigInt.succ x)).*)*)
+(*We in fact need 2 counters: one for identifiers and one
+  for hash consing. Can we reduce duplication and still extract OK?*)
+(*This is a little trick for extraction*)
+Definition hashctr := ctr.
+Definition hashctr_get: hashctr CoqBigInt.t := ctr_get.
+Definition hashctr_ret {a: Type} (x: a) : hashctr a := ctr_ret x.
+Definition hashctr_bnd {a b: Type} (f: a -> ctr b) (x: ctr a) := 
+  ctr_bnd f x.
+Definition new_hashctr : hashctr unit := new_ctr.
+Definition incr_hashctr : hashctr unit := incr.
