src/util/Hashcons.v
@@ -1,0 +1,31 @@
+(*The file name is a lie: we don't (yet?) implement hash consing.
+  But we provide such a (partial) interface*)
+Require Import StateMonad.
+
+Module Type HashedType.
+Parameter t : Type.
+Parameter equal : t -> t -> bool.
+(*Parameter hash : t -> CoqBigInt.t.*) (*We don't need a hash function yet*)
+Parameter tag : CoqBigInt.t -> t -> t.
+End HashedType.
+
+(*A very limited (and fake) version of the interface*)
+Module Type S.
+Parameter t : Type.
+Parameter hashcons : t -> hashctr t.
+End S.
+
+Module Make (H: HashedType) <: S.
+Definition t := H.t.
+
+Definition next_tag : ctr_unit := new_hashctr.
+
+(*this is NOT hashconsing - it always produces a new tag*)
+Definition hashcons (d: t) : hashctr t :=
+  hashctr_bnd (fun i => 
+    let d1 := H.tag i d in
+    hashctr_bnd (fun _ => hashctr_ret d1) 
+      incr_hashctr
+  ) (hashctr_get).
+
+End Make.
