src/util/Weakhtbl.v
@@ -1,0 +1,12 @@
+(*From Weakhtbl - tiny subset*)
+Require CoqBigInt.
+
+Local Definition tag := CoqBigInt.t.
+
+(*NOTE: start counters at 1*)
+Definition dummy_tag : tag := CoqBigInt.zero.
+
+(*We enforce the invariant that all values are nonnegative*)
+Definition tag_hash (k: tag) := k.
+
+Definition create_tag : CoqBigInt.t -> tag := fun x => x.
